Feeling stuck with Hoas

src/Hoas.v
@@ -140,42 +140,54 @@ Inductive Closed : forall t, Exp t -> Prop :=
 
 Axiom closed : forall t (E : Exp t), Closed E.
 
+Ltac my_subst :=
+  repeat match goal with
+           | [ x : type |- _ ] => subst x
+         end.
+
 Ltac my_crush' :=
-  crush;
+  crush; my_subst;
   repeat (match goal with
             | [ H : _ |- _ ] => generalize (inj_pairT2 _ _ _ _ _ H); clear H
-          end; crush).
+          end; crush; my_subst).
+
+Ltac equate_conj F G :=
+  match constr:(F, G) with
+    | (_ ?x1, _ ?x2) => constr:(x1 = x2)
+    | (_ ?x1 ?y1, _ ?x2 ?y2) => constr:(x1 = x2 /\ y1 = y2)
+    | (_ ?x1 ?y1 ?z1, _ ?x2 ?y2 ?z2) => constr:(x1 = x2 /\ y1 = y2 /\ z1 = z2)
+    | (_ ?x1 ?y1 ?z1 ?u1, _ ?x2 ?y2 ?z2 ?u2) => constr:(x1 = x2 /\ y1 = y2 /\ z1 = z2 /\ u1 = u2)
+    | (_ ?x1 ?y1 ?z1 ?u1 ?v1, _ ?x2 ?y2 ?z2 ?u2 ?v2) => constr:(x1 = x2 /\ y1 = y2 /\ z1 = z2 /\ u1 = u2 /\ v1 = v2)
+  end.
 
 Ltac my_crush :=
   my_crush';
-  try (match goal with
-         | [ H : ?F = ?G |- _ ] =>
-           match goal with
-             (*| [ _ : F (fun _ => unit) = G (fun _ => unit) |- _ ] => fail 1*)
-             | _ =>
-               let H' := fresh "H'" in
-                 assert (H' : F (fun _ => unit) = G (fun _ => unit)); [ congruence
-                   | discriminate || injection H' ];
-                 clear H'
-           end
-       end; my_crush');
-  repeat match goal with
-           | [ H : ?F = ?G, H2 : ?X (fun _ => unit) = ?Y (fun _ => unit) |- _ ] =>
-             match X with
-               | Y => fail 1
-               | _ =>
-                 assert (X = Y); [ unfold Exp; apply ext_eq; intro var;
-                   let H' := fresh "H'" in
-                     assert (H' : F var = G var); [ congruence
-                       | match type of H' with
-                           | ?X = ?Y =>
-                             let X := eval hnf in X in
-                               let Y := eval hnf in Y in
-                                 change (X = Y) in H'
-                         end; injection H'; clear H'; my_crush' ]
-                   | my_crush'; clear H2 ]
-             end
-         end.
+  repeat (match goal with
+            | [ H : ?F = ?G |- _ ] =>
+              (let H' := fresh "H'" in
+                assert (H' : F (fun _ => unit) = G (fun _ => unit)); [ congruence
+                  | discriminate || injection H'; clear H' ];
+                my_crush';
+                repeat match goal with
+                         | [ H : context[fun _ => unit] |- _ ] => clear H
+                       end;
+                match type of H with
+                  | ?F = ?G =>
+                    let ec := equate_conj F G in
+                      let var := fresh "var" in
+                        assert ec; [ intuition; unfold Exp; apply ext_eq; intro var;
+                          assert (H' : F var = G var); try congruence;
+                            match type of H' with
+                              | ?X = ?Y =>
+                                let X := eval hnf in X in
+                                  let Y := eval hnf in Y in
+                                    change (X = Y) in H'
+                            end; injection H'; my_crush'; tauto
+                          | intuition; subst ]
+                end);
+              clear H
+          end; my_crush');
+  my_crush'.
 
 Hint Extern 1 (_ = _ @ _) => simpl.
 
@@ -342,6 +354,386 @@ Section cfold.
 End cfold.
 
 Definition Cfold t (E : Exp t) : Exp t := fun _ => cfold (E _).
+Definition Cfold1 t1 t2 (E : Exp1 t1 t2) : Exp1 t1 t2 := fun _ x => cfold (E _ x).
+
+Lemma fold_Cfold : forall t (E : Exp t),
+  (fun _ => cfold (E _)) = Cfold E.
+  reflexivity.
+Qed.
+
+Hint Rewrite fold_Cfold : fold.
+
+Lemma fold_Cfold1 : forall t1 t2 (E : Exp1 t1 t2),
+  (fun _ x => cfold (E _ x)) = Cfold1 E.
+  reflexivity.
+Qed.
+
+Lemma fold_Subst_Cfold1 : forall t1 t2 (E : Exp1 t1 t2) (V : Exp t1),
+  (fun _ => flatten (cfold (E _ (V _))))
+  = Subst V (Cfold1 E).
+  reflexivity.
+Qed.
+
+Axiom cheat : forall T, T.
+
+
+Lemma fold_Const : forall n, (fun _ => Const' n) = Const n.
+  reflexivity.
+Qed.
+Lemma fold_Plus : forall (E1 E2 : Exp _), (fun _ => Plus' (E1 _) (E2 _)) = Plus E1 E2.
+  reflexivity.
+Qed.
+Lemma fold_App : forall dom ran (F : Exp (dom --> ran)) (X : Exp dom),
+  (fun _ => App' (F _) (X _)) = App F X.
+  reflexivity.
+Qed.
+Lemma fold_Abs : forall dom ran (B : Exp1 dom ran),
+  (fun _ => Abs' (B _)) = Abs B.
+  reflexivity.
+Qed.
+
+Hint Rewrite fold_Const fold_Plus fold_App fold_Abs : fold.
+
+Lemma fold_Subst : forall t1 t2 (E1 : Exp1 t1 t2) (V : Exp t1),
+  (fun _ => flatten (E1 _ (V _))) = Subst V E1.
+  reflexivity.
+Qed.
+
+Hint Rewrite fold_Subst : fold.
+
+Definition ExpN (G : list type) (t : type) := forall var, hlist var G -> exp var t.
+
+Definition ConstN G (n : nat) : ExpN G Nat :=
+  fun _ _ => Const' n.
+Definition VarN G t (m : member t G) : ExpN G t := fun _ s => Var (hget s m).
+Definition PlusN G (E1 E2 : ExpN G Nat) : ExpN G Nat :=
+  fun _ s => Plus' (E1 _ s) (E2 _ s).
+Definition AppN G dom ran (F : ExpN G (dom --> ran)) (X : ExpN G dom) : ExpN G ran :=
+  fun _ s => App' (F _ s) (X _ s).
+Definition AbsN G dom ran (B : ExpN (dom :: G) ran) : ExpN G (dom --> ran) :=
+  fun _ s => Abs' (fun x => B _ (x ::: s)).
+
+Inductive ClosedN : forall G t, ExpN G t -> Prop :=
+| CConstN : forall G b,
+  ClosedN (ConstN G b)
+| CPlusN : forall G (E1 E2 : ExpN G _),
+  ClosedN E1
+  -> ClosedN E2
+  -> ClosedN (PlusN E1 E2)
+| CAppN : forall G dom ran (E1 : ExpN G (dom --> ran)) E2,
+  ClosedN E1
+  -> ClosedN E2
+  -> ClosedN (AppN E1 E2)
+| CAbsN : forall G dom ran (E1 : ExpN (dom :: G) ran),
+  ClosedN E1
+  -> ClosedN (AbsN E1).
+
+Axiom closedN : forall G t (E : ExpN G t), ClosedN E.
+
+Hint Resolve closedN.
+
+Section Closed1.
+  Variable xt : type.
+
+  Definition Const1 (n : nat) : Exp1 xt Nat :=
+    fun _ _ => Const' n.
+  Definition Var1 : Exp1 xt xt := fun _ x => Var x.
+  Definition Plus1 (E1 E2 : Exp1 xt Nat) : Exp1 xt Nat :=
+    fun _ s => Plus' (E1 _ s) (E2 _ s).
+  Definition App1 dom ran (F : Exp1 xt (dom --> ran)) (X : Exp1 xt dom) : Exp1 xt ran :=
+    fun _ s => App' (F _ s) (X _ s).
+  Definition Abs1 dom ran (B : forall var, var dom -> Exp1 xt ran) : Exp1 xt (dom --> ran) :=
+    fun _ s => Abs' (fun x => B _ x _ s).
+
+  Inductive Closed1 : forall t, Exp1 xt t -> Prop :=
+  | CConst1 : forall b,
+    Closed1 (Const1 b)
+  | CPlus1 : forall E1 E2,
+    Closed1 E1
+    -> Closed1 E2
+    -> Closed1 (Plus1 E1 E2)
+  | CApp1 : forall dom ran (E1 : Exp1 _ (dom --> ran)) E2,
+    Closed1 E1
+    -> Closed1 E2
+    -> Closed1 (App1 E1 E2)
+  | CAbs1 : forall dom ran (E1 : forall var, var dom -> Exp1 _ ran),
+    Closed1 (Abs1 E1).
+
+  Axiom closed1 : forall t (E : Exp1 xt t), Closed1 E.
+End Closed1.
+
+Hint Resolve closed1.
+
+Definition CfoldN G t (E : ExpN G t) : ExpN G t := fun _ s => cfold (E _ s).
+
+Theorem fold_CfoldN : forall G t (E : ExpN G t),
+  (fun _ s => cfold (E _ s)) = CfoldN E.
+  reflexivity.
+Qed.
+
+Definition SubstN t1 G t2 (E1 : ExpN G t1) (E2 : ExpN (G ++ t1 :: nil) t2) : ExpN G t2 :=
+  fun _ s => flatten (E2 _ (hmap (@Var _) s +++ E1 _ s ::: hnil)).
+
+Lemma fold_SubstN : forall t1 G t2 (E1 : ExpN G t1) (E2 : ExpN (G ++ t1 :: nil) t2),
+  (fun _ s => flatten (E2 _ (hmap (@Var _) s +++ E1 _ s ::: hnil))) = SubstN E1 E2.
+  reflexivity.
+Qed.
+
+Hint Rewrite fold_CfoldN fold_SubstN : fold.
+
+Ltac ssimp := unfold Subst, Cfold, CfoldN, SubstN in *; simpl in *; autorewrite with fold in *;
+  repeat match goal with
+           | [ xt : type |- _ ] =>
+             rewrite (@fold_Subst xt) in *
+         end;
+  autorewrite with fold in *.
+
+Ltac uiper :=
+  repeat match goal with
+           | [ H : _ = _ |- _ ] =>
+             generalize H; subst; intro H; rewrite (UIP_refl _ _ H)
+         end.
+
+Section eq_arg.
+  Variable A : Type.
+  Variable B : A -> Type.
+
+  Variable x : A.
+
+  Variables f g : forall x, B x.
+  Hypothesis Heq : f = g.
+
+  Theorem eq_arg : f x = g x.
+    congruence.
+  Qed.
+End eq_arg.
+
+Implicit Arguments eq_arg [A B f g].
+
+(*Lemma Cfold_Subst_comm : forall G t (E : ExpN G t),
+  ClosedN E
+  -> forall t1 G' (pf : G = G' ++ t1 :: nil) V,
+    CfoldN (SubstN V (match pf in _ = G return ExpN G _ with refl_equal => E end))
+    = SubstN (CfoldN V) (CfoldN (match pf in _ = G return ExpN G _ with refl_equal => E end)).
+  induction 1; my_crush; uiper; ssimp; crush;
+    unfold ExpN; do 2 ext_eq.
+
+  generalize (eq_arg x0 (eq_arg x (IHClosedN1 _ _ (refl_equal _) V))).
+  generalize (eq_arg x0 (eq_arg x (IHClosedN2 _ _ (refl_equal _) V))).
+  crush.
+
+  match goal with
+    | [ |- _ = flatten (match ?E with
+                          | Const' _ => _
+                          | Plus' _ _ => _
+                          | Var _ _ => _
+                          | App' _ _ _ _ => _
+                          | Abs' _ _ _ => _
+                        end) ] => dep_destruct E
+  end; crush.
+
+  match goal with
+    | [ |- _ = flatten (match ?E with
+                          | Const' _ => _
+                          | Plus' _ _ => _
+                          | Var _ _ => _
+                          | App' _ _ _ _ => _
+                          | Abs' _ _ _ => _
+                        end) ] => dep_destruct E
+  end; crush.
+
+  match goal with
+    | [ |- match ?E with
+             | Const' _ => _
+             | Plus' _ _ => _
+             | Var _ _ => _
+             | App' _ _ _ _ => _
+             | Abs' _ _ _ => _
+           end = _ ] => dep_destruct E
+  end; crush.
+  rewrite <- H2.
+
+  dep_destruct e.
+  intro 
+  
+
+  apply cheat.
+
+  unfold ExpN; do 2 ext_eq.
+  generalize (eq_arg x0 (eq_arg x (IHClosedN1 _ _ (refl_equal _) V))).
+  generalize (eq_arg x0 (eq_arg x (IHClosedN2 _ _ (refl_equal _) V))).
+  congruence.
+
+  unfold ExpN; do 2 ext_eq.
+  f_equal.
+  ext_eq.
+  exact (eq_arg (x1 ::: x0) (eq_arg x (IHClosedN _ (dom :: G') (refl_equal _) (fun _ s => V _ (snd s))))).
+Qed.*)
+
+Lemma Cfold_Subst' : forall t (E V' : Exp t),
+  E ===> V'
+  -> forall G xt (V : ExpN G xt) B, E = SubstN V B
+    -> ClosedN B
+    -> Subst (Cfold V) (Cfold1 B) ===> Cfold V'.
+  induction 1; inversion 2; my_crush; ssimp.
+
+  auto.
+
+  apply cheat.
+
+  my_crush.
+  econstructor.
+  instantiate (1 := Cfold1 B).
+  unfold Subst, Cfold1 in *; eauto.
+  unfold Subst, Cfold1 in *; eauto.
+  unfold Subst, Cfold; eauto.
+
+  my_crush; ssimp.
+  
+  
+    
+
+  Lemma Cfold_Subst' : forall t (B : Exp1 xt t),
+    Closed1 B
+    -> forall V', Subst V B ===> V'
+      -> Subst (Cfold V) (Cfold1 B) ===> Cfold V'.
+    induction 1; my_crush; ssimp.
+
+    inversion H; my_crush.
+
+    apply cheat.
+
+    inversion H1; my_crush.
+    econstructor.
+    instantiate (1 := Cfold1 B).
+    eauto.
+    change (Abs (Cfold1 B)) with (Cfold (Abs B)).
+    auto.
+    eauto.
+    eauto.
+
+    apply IHClosed1_1.
+    eauto.
+
+    match goal with
+      | [ (*H : ?F = ?G,*) H2 : ?X (fun _ => unit) = ?Y _ _ _ _ (fun _ => unit) |- _ ] =>
+        idtac(*match X with
+          | Y => fail 1
+          | _ =>
+            idtac(*assert (X = Y); [ unfold Exp; apply ext_eq; intro var;
+              let H' := fresh "H'" in
+                assert (H' : F var = G var); [ congruence
+                  | match type of H' with
+                      | ?X = ?Y =>
+                        let X := eval hnf in X in
+                          let Y := eval hnf in Y in
+                            change (X = Y) in H'
+                    end; injection H'; clear H'; my_crush' ]
+              | my_crush'; clear H2 ]*)
+        end*)
+    end.
+
+    clear H5 H3.
+    my_crush.
+
+
+    unfold Subst in *; simpl in *; autorewrite with fold in *.
+    
+
+  Check fold_Subst.
+  
+  repeat rewrite (@fold_Subst t1) in *.
+
+  simp (Subst (t2 := Nat) V).
+  
+
+  induction 1; my_crush.
+End Exp1.
+
+Axiom closed1 : forall t1 t2 (E : Exp1 t1 t2), Closed1 E.
+
+
+
+Lemma Cfold_Subst' : forall t1 (V : Exp t1) t2 (B : Exp1 t1 t2),
+  Closed1 B
+  -> forall V', Subst V B ===> V'
+    -> Subst (Cfold V) (Cfold1 B) ===> Cfold V'.
+  induction 1; my_crush.
+
+  unfold Subst in *; simpl in *; autorewrite with fold in *.
+  inversion H; my_crush.
+
+  unfold Subst in *; simpl in *; autorewrite with fold in *.
+  Check fold_Subst.
+  
+  repeat rewrite (@fold_Subst t1) in *.
+
+  simp (Subst (t2 := Nat) V).
+  
+
+  induction 1; my_crush.
+
+Theorem Cfold_Subst : forall t1 t2 (V : Exp t1) B (V' : Exp t2),
+  Subst V B ===> V'
+  -> Subst (Cfold V) (Cfold1 B) ===> Cfold V'.
+
+Theorem Cfold_correct : forall t (E V : Exp t),
+  E ===> V
+  -> Cfold E ===> Cfold V.
+  induction 1; unfold Cfold in *; crush; simp; auto.
+
+  simp.
+  simp.
+  apply cheat.
+
+  simp.
+  econstructor; eauto.
+  
+
+
+  match goal with
+    | [ |- ?E ===> ?V ] =>
+      try simp1 ltac:(fun E' => change (E' ===> V));
+        try match goal with
+              | [ |- ?E' ===> _ ] =>
+                simp1 ltac:(fun V' => change (E' ===> V'))
+            end
+    | [ H : ?E ===> ?V |- _ ] =>
+      try simp1 ltac:(fun E' => change (E' ===> V) in H);
+        try match type of H with
+              | ?E' ===> _ =>
+                simp1 ltac:(fun V' => change (E' ===> V') in H)
+            end
+  end.
+  simp.
+
+  let H := IHBigStep1 in
+  match type of H with
+    | ?E ===> ?V => 
+      try simp1 ltac:(fun E' => change (E' ===> V) in H);
+        try match type of H with
+          | ?E' ===> _ =>
+            simp1 ltac:(fun V' => change (E' ===> V') in H)
+        end
+  end.
+
+try simp1 ltac:(fun E' => change (E' ===> V) in H)
+  end.
+
+  simp.
+
+  try simp1 ltac:(fun E' => change (fun H : type -> Type => cfold (E1 H)) with E' in IHBigStep1).
+    try simp1 ltac:(fun V' => change (fun H : type -> Type =>
+      Abs' (dom:=dom) (fun x : H dom => cfold (B H x))) with V' in IHBigStep1).
+  
+  simp1 ltac:(fun E => change ((fun H : type -> Type => cfold (E1 H)) ===> E) in IHBigStep1).
+
+  change ((fun H : type -> Type => cfold (E1 H)) ===> Abs (fun _ x => cfold (B _ x))) in IHBigStep1.
+    (fun H : type -> Type =>
+      Abs' (dom:=dom) (fun x : H dom => cfold (B H x)))
+
+  fold Cfold.
+
 
 
 Definition ExpN (G : list type) (t : type) := forall var, hlist var G -> exp var t.
